src/tutorial/Example4.v
@@ -1,0 +1,291 @@
+From Tutorial Require Import sflib.
+From Paco Require Import paco.
+From Tutorial Require Import Refinement ITreeLib.
+From Coq Require Import Strings.String List.
+From Tutorial Require Import Imp ITreeLang FiniteSimulation.
+From Coq Require Import Logic.Eqdep.
+
+Set Implicit Arguments.
+
+(** Example 4: ITree version of Example 1.
+    We prove the same refinements as in Example1.v,
+    but using the ITree-based semantics from ITreeLang.v. *)
+
+(** Normalization tactic for ITree goals.
+    [cbn] + repeated rewriting of bind laws and trigger. *)
+Ltac norm :=
+  cbn;
+  repeat (try rewrite bind_trigger;
+          try rewrite bind_bind; try rewrite bind_ret_l;
+          try rewrite bind_tau; try rewrite bind_vis;
+          cbn).
+
+(** Handle dependent equality from [inv] on Vis steps.
+    When inverting an [ITree_step] on a [Vis] node, Coq produces
+    a [sigT] equality that needs [inj_pair2] (axiom K) to resolve. *)
+Ltac dep_subst :=
+  repeat match goal with
+  | [H: existT _ _ _ = existT _ _ _ |- _] =>
+      apply inj_pair2 in H; try subst
+  end.
+
+
+Section DEMO.
+
+  Definition src0 : com := <{ ret 0 }>.
+  Definition tgt0 : com := <{ "x" := (1 + 1); "y" := (2 * 1 - "x"); ret "y" }>.
+
+  Goal refines (ITree_Program_Mem src0) (ITree_Program_Mem tgt0).
+  Proof.
+    apply adequacy.
+    unfold simulation, ITree_Program_Mem, ITree_STS_Mem, ITree_STS, src0, tgt0, denote_program.
+    norm.
+    (* tgt = tau;; tau;; Ret 0, src = Ret 0 *)
+    econs 4. { ss. }
+    ss. i. inv H. ss. split; auto. norm.
+    econs 4. { ss. }
+    ss. i. inv H. ss. split; auto. norm.
+    econs 1; ss.
+  Qed.
+
+End DEMO.
+
+Section EX.
+
+  (* Ex1. External calls are observable. *)
+  Definition src1 : com :=
+    <{ "a" :=@ "print" <[0 : aexp]>; ret "a" }>.
+
+  Definition tgt1 : com :=
+    <{ "x" := 0; "y" :=@ "print" <["x" : aexp]>; ret "y" }>.
+
+  Goal refines (ITree_Program_Mem src1) (ITree_Program_Mem tgt1).
+  Proof.
+    apply adequacy.
+    unfold simulation, ITree_Program_Mem, ITree_STS_Mem, ITree_STS, src1, tgt1, denote_program.
+    norm.
+    (* tgt = tau;; vis (Observe "print" [0]) ..., src = vis (Observe "print" [0]) ... *)
+    econs 4; ss.
+    i. inv H. ss. split; auto.
+    (* Both have vis (Observe "print" [0]) at head — observable step *)
+    econs 2; ss.
+    i. inv H. dep_subst.
+    ss. split; auto.
+    esplits.
+    { eapply ITree_step_observe. }
+    norm.
+    (* sim (Mem.init, tau;; Ret retv) (Mem.init, tau;; Ret retv) *)
+    econs 4; ss.
+    i. inv H. ss. split; auto.
+    econs 3; ss. esplits.
+    - econs.
+    - ss.
+    - econs 1; ss.
+  Qed.
+
+
+  (* Ex2. If semantics is given by ITree_STS_Mem, memory accesses are also observable. *)
+  Definition src2 : com :=
+    <{ &<1> := 5; "a" := &<1>; ret "a" }>.
+
+  Definition tgt2 : com :=
+    <{ "x" := 2; &<1> := ("x" + 3); "y" := &<1>; ret "y" }>.
+
+  Goal refines (ITree_Program_Mem src2) (ITree_Program_Mem tgt2).
+  Proof.
+    apply adequacy.
+    unfold simulation, ITree_Program_Mem, ITree_STS_Mem, ITree_STS, src2, tgt2, denote_program.
+    norm.
+    econs 4; ss. i. inv H. ss. split; auto. norm.
+    econs 2; ss. i. inv H. dep_subst.
+    ss. split; auto.
+    eexists. split.
+    { eapply ITree_step_store. }
+    norm.
+    econs 4; ss. i. inv H. ss. split; auto. norm.
+    econs 3; ss. esplits.
+    - econs.
+    - ss.
+    - norm.
+      econs 2; ss. i. inv H. dep_subst.
+      + ss. split; auto.
+        eexists. split.
+        { eapply ITree_step_load. ss. }
+        norm.
+        econs 4; ss. i. inv H. ss. split; auto. norm.
+        econs 3; ss. esplits.
+        * econs.
+        * ss.
+        * norm. econs 1; ss.
+      + ss.
+  Qed.
+
+  (* Ex2'. With ITree_STS_Ext, memory accesses are silent. *)
+  Definition src2' : com :=
+    <{ ret 5 }>.
+
+  Goal refines (ITree_Program_Ext src2') (ITree_Program_Ext tgt2).
+  Proof.
+    apply adequacy.
+    unfold simulation, ITree_Program_Ext, ITree_STS_Ext, ITree_STS, src2', tgt2, denote_program.
+    norm.
+    econs 4; ss. i. inv H. ss. split; auto. norm.
+    econs 4; ss. i. inv H. dep_subst. ss. split; auto. norm.
+    econs 4; ss. i. inv H. ss. split; auto. norm.
+    econs 4; ss. i. inv H; dep_subst; ss; split; auto; norm.
+    simpl in LOAD. inv LOAD.
+    econs 4; ss. i. inv H. ss. split; auto. norm.
+    econs 1; ss.
+  Qed.
+
+
+  (* Ex3. If the source can exhibit UB, refinement always holds. *)
+  Definition src3 : com :=
+    <{ ret "a" }>.
+
+  Goal forall tgt, refines (ITree_Program_Mem src3) (ITree_Program_Mem tgt).
+  Proof.
+    i. apply adequacy.
+    unfold simulation, ITree_Program_Mem, ITree_STS_Mem, ITree_STS, src3, denote_program.
+    norm.
+    econs 5. ss.
+  Qed.
+
+
+  (* Ex4. If a loop always terminates, we can prove it by induction. *)
+  Definition src4 : com :=
+    <{ ret 0 }>.
+
+  Definition tgt4 : com :=
+    <{ "x" := 100;
+       while ("x")
+       do ("x" := ("x" - 1))
+       end;
+       ret "x"
+    }>.
+
+  Goal refines (ITree_Program_Mem src4) (ITree_Program_Mem tgt4).
+  Proof.
+    apply adequacy.
+    unfold simulation, ITree_Program_Mem, ITree_STS_Mem, ITree_STS, src4, tgt4, denote_program.
+    norm.
+    econs 4; ss. i. inv H. ss. split; auto.
+    match goal with
+    | |- sim _ (_, ITree.bind (ITree.iter ?body ?init) ?k) =>
+        enough (LOOP: forall n r0, Reg.read r0 "x" = Some n ->
+          @sim _ ekind_memory _ ITree_step ITree_sort
+            (Mem.init, Ret 0) (Mem.init, ITree.bind (ITree.iter body r0) k))
+    end.
+    { eapply LOOP. ss. }
+    induction n; intros r0 Hx.
+    - rewrite unfold_iter_eq. norm. rewrite Hx. norm.
+      econs 4; ss. i. inv H. ss. split; auto. norm. rewrite Hx. norm.
+      econs 1; ss.
+    - rewrite unfold_iter_eq. norm. rewrite Hx. norm.
+      econs 4; ss. i. inv H. ss. split; auto.
+      apply IHn. ss. rewrite PeanoNat.Nat.sub_0_r. ss.
+  Qed.
+
+End EX.
+
+Section DIV.
+
+  (* DIV1. We can prove the following refinement, which always terminates. *)
+  Definition src5 : com :=
+    <{ "x" := 100;
+       while ("x")
+       do ("a" :=@ "print" <["x" : aexp]>;
+           "x" := ("x" - 1))
+       end;
+       ret "x"
+    }>.
+
+  Definition tgt5 : com :=
+    <{ "x" := 100;
+       while ("x")
+       do ("a" :=@ "print" <["x" : aexp]>;
+           "x" := ("x" - 1))
+       end;
+       ret "x"
+    }>.
+
+  Goal refines (ITree_Program_Ext src5) (ITree_Program_Ext tgt5).
+  Proof.
+    apply adequacy.
+    unfold simulation, ITree_Program_Ext, ITree_STS_Ext, ITree_STS, src5, tgt5, denote_program.
+    norm.
+    (* Initial tau: step tgt then src *)
+    econs 4; ss. i. inv H. ss. split; auto.
+    econs 3; ss. esplits.
+    - econs.
+    - ss.
+    - norm.
+      match goal with
+      | |- sim (_, ITree.bind (ITree.iter ?body ?init) ?k)
+               (_, ITree.bind (ITree.iter ?body' ?init') ?k') =>
+          enough (LOOP: forall n r0, Reg.read r0 "x" = Some n ->
+            @sim _ ekind_external _ ITree_step ITree_sort
+              (Mem.init, ITree.bind (ITree.iter body r0) k)
+              (Mem.init, ITree.bind (ITree.iter body' r0) k'))
+      end.
+      { eapply LOOP. ss. }
+      induction n; intros r0 Hx.
+      + (* n = 0: loop exits *)
+        rewrite !unfold_iter_eq. norm. rewrite Hx. norm.
+        econs 4; ss. i. inv H. ss. split; auto.
+        econs 3; ss. esplits.
+        * econs.
+        * ss.
+        * norm. rewrite Hx. norm.
+          econs 1; ss.
+      + (* n = S n: loop body with external call *)
+        rewrite !unfold_iter_eq. norm. rewrite Hx. norm.
+        (* observable: Observe "print" [S n] *)
+        econs 2; ss. i. inv H. dep_subst.
+        ss. split; auto.
+        esplits.
+        { eapply ITree_step_observe. }
+        (* After observe, Reg.read was unfolded by cbn, fix Hx *)
+        unfold Reg.read in Hx. norm. rewrite Hx. norm.
+        (* step both through tau *)
+        econs 4; ss. i. inv H. ss. split; auto.
+        econs 3; ss. esplits.
+        * econs.
+        * ss.
+        * norm.
+          (* step both through another tau *)
+          econs 4; ss. i. inv H. ss. split; auto.
+          econs 3; ss. esplits.
+          { econs. }
+          { ss. }
+          norm.
+          apply IHn.
+          unfold Reg.read, Reg.write. ss.
+          rewrite PeanoNat.Nat.sub_0_r. ss.
+  Qed.
+
+
+  (* DIV2. We can't prove the following refinement because it can diverge. 
+    See Example1.v's DIV2. *)
+  Definition src6 : com :=
+    <{ "x" := 100;
+       while ("x")
+       do ("x" := AAny)
+       end;
+       ret "x"
+    }>.
+
+  Definition tgt6 : com :=
+    <{ "x" := 100;
+       while ("x")
+       do ("x" := AAny)
+       end;
+       ret "x"
+    }>.
+
+  Goal refines (ITree_Program_Ext src6) (ITree_Program_Ext tgt6).
+  Proof.
+  (* We can't prove this right now. Try to prove using induction, and see where it fails. *)
+  Abort.
+
+End DIV.
